cava2/Components/RealignMaskedFifoProperties.v
@@ -1,0 +1,865 @@
+(****************************************************************************)
+(* Copyright 2021 The Project Oak Authors                                   *)
+(*                                                                          *)
+(* Licensed under the Apache License, Version 2.0 (the "License")           *)
+(* you may not use this file except in compliance with the License.         *)
+(* You may obtain a copy of the License at                                  *)
+(*                                                                          *)
+(*     http://www.apache.org/licenses/LICENSE-2.0                           *)
+(*                                                                          *)
+(* Unless required by applicable law or agreed to in writing, software      *)
+(* distributed under the License is distributed on an "AS IS" BASIS,        *)
+(* WITHOUT WARRANTIES OR CONDITIONS OF ANY KIND, either express or implied. *)
+(* See the License for the specific language governing permissions and      *)
+(* limitations under the License.                                           *)
+(****************************************************************************)
+
+Require Import Coq.Arith.PeanoNat.
+Require Import Coq.micromega.Lia.
+Require Import Coq.NArith.NArith.
+Require Import Coq.ZArith.ZArith.
+Require Import Coq.Lists.List.
+
+Require Import coqutil.Tactics.Tactics.
+
+Require Import Cava.Util.List.
+Require Import Cava.Util.Nat.
+Require Import Cava.Util.Byte.
+Require Import Cava.Util.Tactics.
+Require Import Cava.Util.If.
+
+Require Import Cava.Types.
+Require Import Cava.Expr.
+Require Import Cava.ExprProperties.
+Require Import Cava.Primitives.
+Require Import Cava.Semantics.
+Require Import Cava.Invariant.
+
+Require Import Cava.Components.Fifo.
+Require Import Cava.Components.RealignMasked.
+Require Import Cava.Components.RealignMaskedFifo.
+Require Import Cava.Components.FifoProperties.
+Require Import Cava.Components.RealignMaskedProperties.
+
+Import ListNotations.
+
+Local Open Scope bool.
+Local Open Scope nat.
+Local Open Scope list.
+
+Section RealignMaskedFifo.
+  Context (fifo_size: nat).
+  Context (Hfifo_nz: (1 < fifo_size)%nat).
+
+  Hint Extern 0 (1 < fifo_size) => apply Hfifo_nz : typeclass_instances .
+  Existing Instance fifo_specification.
+  Existing Instance fifo_correctness.
+  Existing Instance realign_specification.
+  Existing Instance realign_correctness.
+  Set Typeclasses Debug.
+
+
+  Lemma concat_bytes_resize xs:
+    length xs <= 4 -> BigEndianBytes.concat_bytes (List.resize Byte.x00 4 xs)
+                 = BigEndianBytes.concat_bytes xs.
+  Admitted.
+
+  Global Instance realign_masked_fifo_invariant
+  : invariant_for (realign_masked_fifo fifo_size) (list N * (bool * list Byte.byte * list Byte.byte)) :=
+      fun state '(fifo_contents, realign_contents)  =>
+        let '(state, (realign_state, fifo_state)) := state in
+        let '(is_last, (out_valid, (out_data, (out_length, (fifo_empty, fifo_full))))) := state in
+
+        fifo_invariant (BitVec 32) fifo_size fifo_state fifo_contents
+        /\ realign_invariant realign_state realign_contents
+        /\ (if fifo_full then length fifo_contents = fifo_size else length fifo_contents < fifo_size)
+        /\ (if fifo_empty then length fifo_contents = 0 else length fifo_contents > 0)
+        .
+
+  Instance realign_masked_fifo_specification
+  : specification_for (realign_masked_fifo fifo_size) (list N * (bool * list Byte.byte * list Byte.byte)) :=
+    {| reset_repr := ([], (false, [], []));
+     update_repr :=
+      fun (input: denote_type (input_of (realign_masked_fifo fifo_size))) '(fifo_contents, realign_contents) =>
+      let '(data_valid, (data, (data_mask, (drain, (consumer_ready, tt))))) := input in
+
+      let fifo_empty := length fifo_contents =? 0 in
+      let fifo_full := length fifo_contents =? fifo_size in
+
+      let realign_input :=
+        (data_valid, (data, (data_mask, (drain && fifo_empty && consumer_ready, (negb fifo_full, tt))))) in
+      let '(realign_valid, realign_data, new_realign_contents) :=
+        update_repr (c:=realign) realign_input realign_contents in
+      let fifo_input :=
+        (realign_valid && negb drain && negb fifo_full, (BigEndianBytes.concat_bytes realign_data, (consumer_ready, tt))) in
+      let new_fifo_contents :=
+        update_repr (c:=fifo (T:=BitVec 32) fifo_size) fifo_input fifo_contents in
+
+      (new_fifo_contents, (realign_valid, realign_data, new_realign_contents));
+
+     precondition :=
+      fun (input: denote_type (input_of (realign_masked_fifo fifo_size))) '(fifo_contents, realign_contents) =>
+
+      let '(data_valid, (data, (data_mask, (drain, (consumer_ready, tt))))) := input in
+
+      let fifo_empty := length fifo_contents =? 0 in
+      let fifo_full := length fifo_contents =? fifo_size in
+
+      let realign_input :=
+        (data_valid, (data, (data_mask, (drain && fifo_empty && consumer_ready, (negb fifo_full, tt))))) in
+      let '(realign_valid, realign_data, new_realign_contents) :=
+        update_repr (c:=realign) realign_input realign_contents in
+      let fifo_input :=
+        (realign_valid && negb drain && negb fifo_full, (BigEndianBytes.concat_bytes realign_data, (consumer_ready, tt))) in
+
+      precondition realign realign_input realign_contents
+      /\ precondition (fifo (T:=BitVec 32) fifo_size) fifo_input fifo_contents
+      ;
+
+     postcondition :=
+      fun input contents (output: denote_type (output_of (realign_masked_fifo fifo_size))) =>
+        True;
+  |}%nat.
+
+  Lemma realign_masked_fifo_invariant_preserved : invariant_preserved (realign_masked_fifo fifo_size).
+  Proof.
+    cbv [invariant_preserved].
+    cbn [absorb_any] in *.
+    destruct input as (data_valid, (data, (data_mask, (drain, (consumer_ready, []))))).
+    destruct state as (state, (realign_state, fifo_state)).
+    destruct state as (is_last, (out_valid, (out_data, (out_length, (fifo_empty, fifo_full))))).
+    intros input state r new_r; subst.
+    simplify_invariant (realign_masked_fifo fifo_size); logical_simplify; intros.
+    cbv [realign_masked_fifo]; stepsimpl; logical_simplify; subst.
+    destruct input as (new_fifo_contents, new_realign_contents); logical_simplify.
+    destruct new_realign_contents as ((new_latched_valid,new_latched_bytes), new_realign_ghost).
+    cbv [precondition] in H.
+    cbv [realign_masked_fifo_specification update_repr] in H.
+    cbn [realign_specification update_repr] in H.
+    logical_simplify.
+
+    repeat (destruct_pair_let; cbn [fst snd]).
+    ssplit.
+    {
+      use_correctness' realign.
+      eapply (invariant_preserved_pf (c:=fifo fifo_size)); cycle 1;
+      simplify_spec (fifo (T:=BitVec 32) fifo_size); eauto.
+      { use_correctness' realign.
+        rewrite H5.
+        cbv [realign_spec].
+        autorewrite with tuple_if; cbn [fst snd]; boolsimpl.
+        simplify_invariant realign; cbv [realign_invariant'] in *; logical_simplify.
+        destruct fifo_full; boolsimpl; eauto.
+
+        destruct (((4 <=? length new_realign_ghost)
+          || drain && fifo_empty && consumer_ready && (1 <=? length new_realign_ghost)) && negb drain);
+          eauto.
+      }
+      cbn [denote_type absorb_any] in *; f_equal; rewrite H5.
+
+      simplify_spec (realign_masked_fifo fifo_size).
+      simplify_spec realign.
+      simplify_spec (fifo (T:=BitVec 32) fifo_size).
+      cbv [realign_update_latched_valid realign_update_latched_bytes realign_spec] in *.
+      autorewrite with tuple_if; cbn [fst snd]; destruct fifo_full; boolsimpl.
+      { destruct (length new_fifo_contents =? fifo_size); boolsimpl; try reflexivity.
+        {
+          revert H4; rewrite H2.
+          destr (fifo_size =? 0); boolsimpl; try lia.
+          destruct ((4 <=? length new_realign_ghost) && negb drain).
+          { intros. lia. }
+          { reflexivity. }
+        }
+      }
+      { destruct (length new_fifo_contents =? fifo_size); boolsimpl; try reflexivity.
+        destruct fifo_empty; destruct (length new_fifo_contents =? 0); boolsimpl; try reflexivity;
+          destruct drain; boolsimpl; try reflexivity;
+          (destr (4 <=? length new_realign_ghost); [|reflexivity]); now rewrite resize_firstn_alt by lia.
+      }
+    }
+    {
+      eapply (invariant_preserved_pf (c:=realign)); eauto.
+      simplify_spec (realign_masked_fifo fifo_size).
+      simplify_spec realign.
+      simplify_invariant realign.
+      cbn [fst snd].
+      cbv [realign_update_latched_valid realign_update_latched_bytes realign_update_state].
+      autorewrite with tuple_if; cbn [fst snd];
+        destruct fifo_full; try rewrite H2; try rewrite Nat.eqb_refl;
+        boolsimpl; try reflexivity.
+      destr (length new_fifo_contents =? fifo_size); try lia.
+      destruct fifo_empty; try rewrite H3; boolsimpl; try reflexivity.
+      destr (length new_fifo_contents =? 0); try lia; boolsimpl.
+      reflexivity.
+    }
+    { admit. }
+    {
+      simplify_spec (realign_masked_fifo fifo_size).
+      simplify_spec realign.
+      assert ( (length new_fifo_contents =? fifo_size) = fifo_full).
+      { destruct fifo_full; subst.
+        { now rewrite Nat.eqb_refl. }
+        { apply Nat.eqb_neq. lia. }
+      }
+      assert ( (length new_fifo_contents =? 0) = fifo_empty).
+      { destruct fifo_empty.
+        { rewrite H3. now rewrite Nat.eqb_refl. }
+        { apply Nat.eqb_neq. lia. }
+      }
+      rewrite H6, H7 in H4.
+      cbn [realign_spec].
+      use_correctness' realign.
+      rewrite H5.
+      boolsimpl.
+      destruct fifo_full; destruct fifo_empty.
+      try rewrite H2, H3, Nat.eqb_refl in *.
+      {
+      rewrite H5.
+      autorewrite with tuple_if.
+      (* autorewrite with tuple_if; cbn [fst snd]; *)
+      cbv
+      destruct fifo_full; try rewrite H2; try rewrite Nat.eqb_refl;
+        boolsimpl; push_length.
+      rewrite
+      use_correctness' (fifo (T:= BitVec 32) fifo_size).
+      cbn [fst snd].
+
+  Admitted.
+
+
+
+
+    logical_simplify.
+    stepsimpl.
+    repeat (destruct_pair_let ; cbn [fst snd]).
+    cbn [denote_type absorb_any] in *.
+    ssplit.
+    {
+      apply step_fifo_invariant with (contents:=fifo_contents).
+      { apply Hfifo_nz. }
+      { now apply Hnew_fifo_contents. }
+      { cbv [fifo_pre].
+        destruct fifo_state as (?,(?,(?,count))).
+        destruct fifo_full.
+        { now boolsimpl. }
+        { boolsimpl.
+          cbv [fifo_invariant] in H.
+          logical_simplify.
+          rewrite H4.
+          match goal with
+          | |- if ?B then _ else _ => destruct B
+          end.
+          { apply H1. }
+          trivial.
+          }
+      }
+      apply H.
+    }
+
+      {
+        destruct r.
+        eapply (invariant_preserved_pf (c:=fifo fifo_size) ).
+        2:{
+          cbn [denote_type] in *; destruct_products.
+          cbn [fst snd].
+          apply H0l. }
+        2:{
+          cbv [precondition fifo_specification].
+          (* cbn [absorb_any] in *. *)
+          pose tktktk as H.
+          (* pose proof (output_correct_pf (c:=realign)). *)
+          cbv [output_correct postcondition realign_specification] in H.
+          cbn [denote_type absorb_any] in *.
+          (* destruct input as (?, (?, (?, (?, (?, ?))))). *)
+          destruct input as (data_valid, (data, (data_mask, (drain, (consumer_ready, []))))).
+          cbn [fst snd].
+          specialize (H
+            (data_valid,
+            (data,
+            (data_mask,
+            (drain && fst (snd (snd (snd (snd (fst state))))) && consumer_ready,
+            (negb (snd (snd (snd (snd (snd (fst state)))))), tt)))))).
+          specialize (H (fst (snd state))).
+          destruct H.
+          (* assert (bool * list Byte.byte * list Byte.byte) by admit. *)
+
+          (* specialize (H H2). *)
+          assert (realign_invariant (fst (snd state)) x) .
+          { cbv [realign_invariant]. destruct x as ((?,?),?).
+            cbv [realign_invariant'].
+            destruct state as (state, (realign_state, fifo_state)).
+            destruct realign_state as (out_valid, (out_data, (out_len, (buff, buff_len)))).
+            cbn [fst snd].
+
+          specialize (H H3).
+          assert (
+           precondition realign
+  (data_valid,
+           (data,
+           (data_mask,
+           (drain && fst (snd (snd (snd (snd (fst state))))) && consumer_ready,
+           (negb (snd (snd (snd (snd (snd (fst state)))))), tt)))))
+             H2) by admit.
+          specialize (H H4).
+          destruct H2 as ((latched_valid, latched_bytes), ghost_state).
+          cbn [absorb_any denote_type] in *.
+          rewrite H.
+          cbv [realign_spec].
+          destruct state as (state, (realign_state, fifo_state)).
+          destruct state as (is_last, (out_valid, (out_data, (out_length, (fifo_empty, fifo_full))))).
+          (* destruct_products. *)
+          autorewrite with tuple_if.
+          cbn [fst snd negb];
+          cbv [fifo_invariant] in H0.
+          destruct fifo_state as (?, (?, (fifo, count))).
+          logical_simplify.
+          destruct fifo_full; boolsimpl.
+          { trivial. }
+          destruct (
+           ((4 <=? length ghost_state)
+            || drain && fifo_empty && consumer_ready && (1 <=? length ghost_state)) && negb drain).
+          { apply H5. }
+          trivial.
+        }
+        cbv [update_repr realign_masked_fifo_specification fifo_specification].
+        destruct input as (data_valid, (data, (data_mask, (drain, (consumer_ready, []))))).
+        destruct state as (state, (realign_state, fifo_state)).
+        destruct state as (is_last, (out_valid, (out_data, (out_length, (fifo_empty, fifo_full))))).
+        cbn [fst snd].
+
+
+
+
+        realign_invariant (fst (snd state)) H2) by admit.
+
+
+        destruct_products.
+        rewrite H2.
+
+        match goal with
+        | |- context [step ?c ?s ?i]=>
+          (* idtac *)
+          (* assert ( realign_invariant d10 p) by admit; *)
+          (* assert ( realign_pre (d, (d0, (d1, (d2 && d8 && fst d3, (negb d9, tt))))) ) by admit; *)
+          (* pose proof (output_correct_pf (c:=c) i s p (ltac:(eauto)) (ltac:(eauto))) *)
+          (* generalize dependent (snd (step c s i)); intros; *)
+          (* simplify_spec c; logical_simplify *)
+        end.
+        destruct p as ((?,?),?).
+        destruct p.
+
+        subst.
+
+
+
+    rewrite (surjective_pairing (step c s i));
+          use_correctness.
+
+        }
+        admit. }
+      {
+        rewrite (surjective_pairing (step c s i));
+
+        use_correctness' realign.
+
+        cbv [ update_repr realign_masked_fifo_specification fifo_specification].
+
+        match goal with
+        | |- context [ step realign ?X ?Y ] =>
+          remember (step realign X Y);
+          pose proof (output_correct_pf (c:=realign) Y X (false, [], l0))
+        end.
+        destruct p as ((?,?),?).
+        intros.
+        cbn [absorb_any] in *.
+        specialize (H X).
+
+        (* simplify_spec (fifo (T:=BitVec 32) fifo_size). *)
+        simplify_spec realign.
+
+        destruct enable; [ | reflexivity ].
+        change (2 ^ 8) with 256 in *. change (2 ^ 16) with 65536 in *.
+        Zify.zify. Z.to_euclidean_division_equations. lia. }
+        repeat (destruct_pair_let; cbn [fst snd]).
+        destruct realign_masked_fifo_specification.
+        destruct fifo_specification.
+        cbv [ update_repr].
+
+      cbv [invariant_preserved]. intros (enable,[]) (data,?) value.
+      intros; subst. simplify_invariant double_counter.
+      cbv [double_counter]. stepsimpl. logical_simplify; subst.
+      repeat use_correctness. stepsimpl.
+      simplify_spec double_counter.
+      ssplit.
+      { eapply (invariant_preserved_pf (c:=counter));
+          [ | solve [eauto] .. ].
+        simplify_spec counter.
+        destruct enable; [ | reflexivity ].
+        change (2 ^ 8) with 256 in *. change (2 ^ 16) with 65536 in *.
+
+
+      use_correctness' (fifo (T:=BitVec 32) fifo_size). stepsimpl.
+      simplify_spec (realign_masked_fifo fifo_size).
+      ssplit.
+
+      (* simplify_invariant double_counter. *)
+      (* simplify_spec double_counter. *)
+      (* intros; logical_simplify; subst. *)
+      (* cbv [double_counter]. stepsimpl. *)
+      (* repeat use_correctness. stepsimpl. *)
+      (* f_equal. *)
+
+
+    (* cbv [fifo_invariant]. cbn [absorb_any]. *)
+    simplify_spec (realign_masked_fifo fifo_size).
+    intros.
+    destruct r.
+    destruct new_r.
+    destruct input as (data_valid, (data, (data_mask, (drain, (consumer_ready, []))))).
+    destruct state as (state, (realign_state, fifo_state)).
+    inversion H; clear H.
+    destruct state as (is_last, (out_valid, (out_data, (out_length, (fifo_empty, fifo_full))))).
+    destruct fifo_state as (?, (?, (?, ?))).
+    subst; intros.
+    logical_simplify.
+    intros.
+    repeat (destruct_pair_let; cbn [fst snd]).
+    cbv [realign_masked_fifo]; stepsimpl.
+    repeat (destruct_pair_let; cbn [fst snd]).
+    (* Check fifo. *)
+    eapply (invariant_preserved_pf (c:=fifo fifo_size)).
+    {
+      cbv [update_repr].
+      cbv [fifo_specification].
+      cbv [fifo_invariant] in H0.
+      (* Set Printing Implicit. *)
+      (* match goal with *)
+      (* | |- context [?X] => *)
+      (*   match X with *)
+      (*   | snd (step realign _ _) => remember X as p *)
+      (*   end *)
+      (* end. *)
+
+      (* revert Heqp. *)
+    (* simplify_spec realign. *)
+
+    (* Existing Instance realign_. *)
+
+    lazymatch goal with
+    | |- context [snd (step realign ?s ?i)] =>
+      find_correctness realign;
+      pose proof (output_correct_pf (c:=realign) i s)
+    end.
+
+    specialize (H (true, [], l0)).
+
+    use_correctness' realign.
+    pose proof (output_correct_pf (c:=realign) _ _ ).
+    generalize dependent (snd (step realign realign_state
+     (data_valid,
+     (data,
+     (data_mask,
+     (drain && fifo_empty && consumer_ready, (negb fifo_full, tt))))))
+    ); intros.
+    revert H.
+    simplify_invariant realign; intros. specialize (H X).  subst. logical_simplify; subst
+    use_correctness' realign.
+
+    stepsimpl.
+
+      cbn [update_repr].
+    eappy
+    kcbn [fst snd].
+    logical_simplify.
+    repeat use_correctness. stepsimpl.
+    ssplit.
+
+
+
+      (* cbv [invariant_preserved]. intros (enable,[]) (data,?) value. *)
+      (* intros; subst. simplify_invariant double_counter. *)
+      (* cbv [double_counter]. stepsimpl. logical_simplify; subst. *)
+      repeat use_correctness. stepsimpl.
+      simplify_spec double_counter.
+      ssplit.
+          [ | solve [eauto] .. ].
+        simplify_spec counter.
+        destruct enable; [ | reflexivity ].
+
+
+
+    cbv [realign_masked_fifo K]. stepsimpl. ; subst; intros.
+    cbv [Fifo.fifo K]; stepsimpl; push_length.
+    autorewrite with Nnat.
+    subst.
+    cbv []
+    intros; logical_simplify; revert H0; subst; intros.
+
+  (* Specification for the 'realign_masked_fifo' component defined in terms of
+   * 'fifo_spec' and 'realign_masked_spec'. *)
+  Definition realign_masked_fifo_spec
+    fifo_contents
+    realign_masked_state
+    (input : denote_type (input_of (var:=denote_type) (realign_masked_fifo fifo_size))) :=
+    let '(data_valid, (data, (data_mask, (drain, (consumer_ready, tt))))) := input in
+
+    let fifo_empty := (length fifo_contents =? 0) in
+    let fifo_full := (length fifo_contents =? fifo_size) in
+
+    let realign_masked_input := (data_valid, (data, (data_mask, ((drain && fifo_empty && consumer_ready), (negb fifo_full, tt))))) in
+
+    let '(realign_maskeded_valid, (realign_maskeded_data, realign_maskeded_length)) :=
+      realign_spec
+        (fst (fst realign_masked_state)) (snd (fst realign_masked_state)) (snd realign_masked_state)
+        realign_masked_input
+    in
+
+    let fifo_input := ( (realign_maskeded_valid && (negb drain) && (negb fifo_full)), (realign_maskeded_data, (consumer_ready, tt))) in
+
+    let new_contents :=
+      fifo_contents_update (BitVec 32) fifo_size
+        fifo_empty fifo_full fifo_contents fifo_input
+    in
+
+    let '(fifo_valid, (fifo_data, (fifo_empty, fifo_full))) :=
+      fifo_spec (BitVec 32) fifo_size
+        fifo_contents new_contents fifo_input in
+
+    let valid :=
+      if drain then fifo_valid || realign_maskeded_valid else fifo_valid in
+    let data :=
+      if drain && negb fifo_valid then realign_maskeded_data
+      else fifo_data in
+    let length :=
+      if drain && negb fifo_valid then realign_maskeded_length
+      else 4%N in
+
+    (valid, (data, (length, (drain && negb fifo_valid && valid, fifo_full)))).
+
+  (* Invariant for the 'realign_masked_fifo' component. *)
+  Definition realign_masked_fifo_invariant
+    fifo_contents realign_masked_contents
+    (state : denote_type (state_of (var:=denote_type) (realign_masked_fifo fifo_size))) :=
+
+    let '(top_state, (realign_masked_state, fifo_state)) := state in
+    let '(is_last, (out_valid, (out_data, (out_length, (fifo_empty, fifo_full))))) := top_state in
+
+    fifo_invariant (BitVec 32) fifo_size fifo_contents fifo_state
+    /\ realign_masked_invariant (fst (fst realign_masked_contents)) (snd (fst realign_masked_contents)) (snd realign_masked_contents) realign_masked_state
+    (* the only additional invariant we preserve is that we respect fifo_full &
+     * fifo_empty *)
+    /\ (if fifo_full then fifo_size = length fifo_contents else length fifo_contents < fifo_size)
+    /\ (if fifo_empty then length fifo_contents = 0 else length fifo_contents <> 0).
+
+
+  (* Precondition for the 'realign_masked_fifo' component. *)
+  Definition realign_masked_fifo_pre
+    (input : denote_type (input_of (realign_masked_fifo fifo_size)))
+    (state: denote_type (state_of (realign_masked_fifo fifo_size)))
+    :=
+    let '(valid, (data, _)) := input in
+    let '(_, (realign_masked_state, fifo_state)) := state in
+    let '(_, (_, (_, count))) := fifo_state in
+    (if valid then N.to_nat count < fifo_size else True)
+    /\ (data < 2 ^ 32)%N.
+
+  (* "fifo" state update, not intended to be readable,
+     discovered mechanically during the proof below. *)
+  Definition realign_masked_fifo_update_fifo_contents
+    fifo_contents
+    (input : denote_type (input_of (realign_masked_fifo fifo_size)))
+    (state : denote_type (state_of (realign_masked_fifo fifo_size))):=
+    fifo_contents_update (BitVec 32) fifo_size (length fifo_contents =? 0)
+      (length fifo_contents =? fifo_size) fifo_contents
+      (fst
+         (snd
+            (step realign_masked (fst (snd state))
+               (fst input,
+               (fst (snd input),
+               (fst (snd (snd input)),
+               (fst (snd (snd (snd input))) &&
+                fst (snd (snd (snd (snd (fst state))))) &&
+                fst (snd (snd (snd (snd input)))),
+               (negb (snd (snd (snd (snd (snd (fst state)))))), tt))))))) &&
+       negb (fst (snd (snd (snd input)))) &&
+       negb (snd (snd (snd (snd (snd (fst state)))))),
+      (fst
+         (snd
+            (snd
+               (step realign_masked (fst (snd state))
+                  (fst input,
+                  (fst (snd input),
+                  (fst (snd (snd input)),
+                  (fst (snd (snd (snd input))) &&
+                   fst (snd (snd (snd (snd (fst state))))) &&
+                   fst (snd (snd (snd (snd input)))),
+                  (negb (snd (snd (snd (snd (snd (fst state)))))), tt)))))))),
+      (fst (snd (snd (snd (snd input)))), tt))).
+
+  (* "realign_masked" state update, not intended to be readable,
+     discovered mechanically during the proof below. *)
+  Definition realign_masked_fifo_update_realign_masked_contents
+    realign_masked_contents
+    (input : denote_type (input_of (realign_masked_fifo fifo_size)))
+    (state : denote_type (state_of (realign_masked_fifo fifo_size))) :=
+    let '(top_state, _) := state in
+    let '(is_last, (out_valid, (out_data, (out_length, (fifo_empty, fifo_full))))) := top_state in
+    ( (
+      realign_masked_update_latched_valid (fst (fst realign_masked_contents)) (snd realign_masked_contents)
+        (fst input,
+        (fst (snd input),
+        (fst (snd (snd input)),
+        (fst (snd (snd (snd input))) && fifo_empty &&
+         fst (snd (snd (snd (snd input)))), (negb fifo_full, tt))))),
+      realign_masked_update_latched_bytes (snd (fst realign_masked_contents)) (snd realign_masked_contents)
+        (fst input,
+        (fst (snd input),
+        (fst (snd (snd input)),
+        (fst (snd (snd (snd input))) && fifo_empty &&
+         fst (snd (snd (snd (snd input)))), (negb fifo_full, tt)))))
+      ),
+      realign_masked_update_state (snd realign_masked_contents)
+        (fst input,
+        (fst (snd input),
+        (fst (snd (snd input)),
+        (fst (snd (snd (snd input))) && fifo_empty &&
+         fst (snd (snd (snd (snd input)))), (negb fifo_full, tt)))))
+    ).
+
+
+  Lemma step_realign_masked_fifo_invariant
+      fifo_contents
+      realign_masked_contents
+      new_fifo_contents
+      new_realign_masked_contents
+      (input : denote_type (input_of (realign_masked_fifo fifo_size)))
+      (state : denote_type (state_of (realign_masked_fifo fifo_size))):
+
+    new_fifo_contents = realign_masked_fifo_update_fifo_contents fifo_contents input state ->
+    new_realign_masked_contents = realign_masked_fifo_update_realign_masked_contents realign_masked_contents input state ->
+
+    realign_masked_fifo_pre input state ->
+    realign_masked_fifo_invariant fifo_contents realign_masked_contents state ->
+    realign_masked_fifo_invariant new_fifo_contents new_realign_masked_contents (fst (step (realign_masked_fifo fifo_size) state input)).
+  Proof.
+    cbv [realign_masked_fifo_invariant realign_masked_fifo].
+    destruct state as (top_state, (realign_masked_state, fifo_state)).
+    destruct realign_masked_state as (x0,(x1,(x2,(x3,x4)))).
+    destruct top_state as (is_last, (out_valid, (out_data, (out_length, (fifo_empty, fifo_full))))).
+
+    intros Hnew_fifo_contents Hnew_realign_masked_contents Hpre H.
+    logical_simplify.
+    stepsimpl.
+    repeat (destruct_pair_let ; cbn [fst snd]).
+    cbn [denote_type absorb_any] in *.
+    ssplit.
+    {
+      apply step_fifo_invariant with (contents:=fifo_contents).
+      { apply Hfifo_nz. }
+      { now apply Hnew_fifo_contents. }
+      { cbv [fifo_pre].
+        destruct fifo_state as (?,(?,(?,count))).
+        destruct fifo_full.
+        { now boolsimpl. }
+        { boolsimpl.
+          cbv [fifo_invariant] in H.
+          logical_simplify.
+          rewrite H4.
+          match goal with
+          | |- if ?B then _ else _ => destruct B
+          end.
+          { apply H1. }
+          trivial.
+          }
+      }
+      apply H.
+    }
+    { eapply step_realign_masked_invariant.
+      { now rewrite Hnew_realign_masked_contents. }
+      { now rewrite Hnew_realign_masked_contents. }
+      { now rewrite Hnew_realign_masked_contents. }
+      { cbv [realign_masked_fifo_pre] in Hpre. cbn in input, fifo_state.
+        destruct_products.
+        now cbn.
+      }
+      { apply H0. }
+    }
+    all:
+      cbn [fst snd];
+      erewrite (step_fifo (BitVec 32) fifo_size) with (new_contents := new_fifo_contents);
+      [ | trivial | now rewrite Hnew_fifo_contents |
+        cbn in input; destruct_products; cbn [fifo_pre fst snd];
+        destruct fifo_full; boolsimpl; try trivial;
+          boolsimpl;
+          cbv [fifo_invariant] in H;
+          logical_simplify;
+          rewrite H4;
+          match goal with
+          | |- if ?B then _ else _ => destruct B
+          end; try trivial
+      |  apply H ].
+    {
+      cbv [fifo_spec]; cbn [fst snd].
+      cbn [denote_type absorb_any] in *.
+      destr (length new_fifo_contents =? fifo_size).
+      { now rewrite E. }
+      { eapply step_fifo_invariant with (new_contents:=new_fifo_contents) in H.
+        { cbv [fifo_invariant] in H.
+          destruct (fst (step (fifo fifo_size) _ _)) as (?, (?, (?, ?))).
+          logical_simplify.
+          cbn [denote_type absorb_any] in *.
+          rewrite <- H4 in E.
+          rewrite <- H4.
+          lia.
+        }
+        { lia. }
+        { rewrite Hnew_fifo_contents. reflexivity. }
+        { cbn [fifo_pre fst snd].
+          destruct_products.
+          cbn in H.
+          destruct fifo_full.
+          { now boolsimpl. }
+          { boolsimpl.
+            cbv [fifo_invariant] in H.
+            logical_simplify.
+            rewrite H4.
+            match goal with
+            | |- if ?B then _ else _ => destruct B
+            end.
+            { apply H1. }
+            trivial.
+          }
+        }
+      }
+    }
+    {
+      cbv [fifo_spec]; cbn [fst snd].
+      cbn [denote_type absorb_any] in *.
+      destr (length new_fifo_contents =? 0).
+      { now rewrite E. }
+      { eapply step_fifo_invariant with (new_contents:=new_fifo_contents) in H.
+        { cbv [fifo_invariant] in H.
+          destruct (fst (step (fifo fifo_size) _ _)) as (?, (?, (?, ?))).
+          logical_simplify.
+          cbn [denote_type absorb_any] in *.
+          rewrite <- H4 in E.
+          rewrite <- H4.
+          lia.
+        }
+        { lia. }
+        { rewrite Hnew_fifo_contents. reflexivity. }
+        { cbn [fifo_pre fst snd].
+          destruct_products.
+          cbn in H.
+          destruct fifo_full.
+          { now boolsimpl. }
+          { boolsimpl.
+            cbv [fifo_invariant] in H.
+            logical_simplify.
+            rewrite H4.
+            match goal with
+            | |- if ?B then _ else _ => destruct B
+            end.
+            { apply H1. }
+            trivial.
+          }
+        }
+      }
+    }
+  Qed.
+
+  Lemma step_realign_masked_fifo
+      fifo_contents
+      realign_masked_contents
+      (input : denote_type (input_of (realign_masked_fifo fifo_size)))
+      (state : denote_type (state_of (realign_masked_fifo fifo_size))):
+
+    realign_masked_fifo_pre input state ->
+    realign_masked_fifo_invariant fifo_contents realign_masked_contents state ->
+    snd (step (realign_masked_fifo fifo_size) state input) = realign_masked_fifo_spec fifo_contents realign_masked_contents input.
+  Proof.
+    intros.
+    destruct state as (top_state, (realign_masked_state, fifo_state)) eqn:?.
+    (* destruct realign_masked_state as (x0,(x1,(x2,(x3,x4)))). *)
+    destruct top_state as (is_last, (out_valid, (out_data, (out_length, (fifo_empty, fifo_full))))).
+    cbn in input, state.
+    cbv [realign_masked_fifo realign_masked_fifo_pre realign_masked_fifo_invariant K] in *.
+    intros. logical_simplify. cbn [fst snd] in *.
+    stepsimpl.
+    repeat (destruct_pair_let; cbn [fst snd]).
+
+    match goal with
+    | |- context [snd (step (fifo (T:=BitVec 32) fifo_size) ?X ?Y) ] =>
+      remember (snd (step (fifo (T:=BitVec 32) fifo_size) X Y)) as stepped_fifo
+    end.
+    match goal with
+    | |- context [ snd (step realign_masked ?X ?Y) ] =>
+      remember (snd (step realign_masked X Y)) as stepped_realign_maskeder
+    end.
+
+    assert (length fifo_contents =? fifo_size = fifo_full).
+    { destruct fifo_full.
+      { rewrite H2. apply Nat.eqb_refl. }
+      { apply Nat.eqb_neq. lia. }
+    }
+    assert (length fifo_contents =? 0 = fifo_empty).
+    { destruct fifo_empty.
+      { rewrite H3. apply Nat.eqb_refl. }
+      { apply Nat.eqb_neq. lia. }
+    }
+
+    cbn [denote_type absorb_any] in *.
+    rewrite <- Heqstepped_realign_maskeder in *.
+    rewrite <- Heqstepped_fifo.
+
+    rewrite step_fifo with
+      (T:=BitVec 32) (fifo_size:=fifo_size)
+      (contents:=fifo_contents)
+      (new_contents:=realign_masked_fifo_update_fifo_contents fifo_contents input state)
+      in Heqstepped_fifo; cycle 1.
+    { trivial. }
+    { subst; reflexivity. }
+    { clear Heqstepped_fifo Heqstepped_realign_maskeder.
+      (* clear stepped_fifo stepped_realign_maskeder. *)
+      cbv [fifo_pre].
+      destruct_products.
+      destruct fifo_full; boolsimpl.
+      { trivial. }
+      {
+        match goal with
+        | |- if ?B then _ else _ => destruct B
+        end; try trivial.
+        cbn in H0.
+        logical_simplify.
+        now rewrite H6.
+      }
+    }
+    { trivial. }
+    cbv [realign_masked_fifo_update_fifo_contents] in *.
+
+    rewrite step_realign_masked with
+      (latched_valid:=fst (fst realign_masked_contents))
+      (latched_bytes:=snd (fst realign_masked_contents))
+      (state_data:=snd realign_masked_contents)
+      in Heqstepped_realign_maskeder, Heqstepped_fifo; cycle 1.
+    { cbn [realign_masked_pre]; destruct_products; cbn; trivial. }
+    { subst; cbn [fst snd ]. trivial. }
+    { cbn [realign_masked_pre]; destruct_products; cbn; trivial. }
+    { subst; cbn [fst snd ]. trivial. }
+
+    cbv [realign_masked_fifo_spec].
+    destruct input as (data_valid, (data, (data_mask, (drain, (consumer_ready, u))))).
+    repeat (destruct_pair_let; cbn [fst snd]).
+    destruct u.
+    cbn [denote_type absorb_any] in *.
+    cbv [realign_masked_fifo_update_fifo_contents] in *.
+    cbn [fst snd] in *.
+    rewrite Heqd in Heqstepped_fifo; cbn [fst snd] in Heqstepped_fifo.
+    rewrite H4 in *.
+    rewrite H5 in *.
+    rewrite <- Heqstepped_realign_maskeder in *.
+    rewrite <- Heqstepped_fifo.
+    clear Heqstepped_realign_maskeder Heqstepped_fifo.
+    reflexivity.
+  Qed.
+End RealignMaskedFifo.
